\documentclass{article}
\usepackage{epsfig}
\pagestyle{empty}
\begin{document}
$(s,\theta,\phi)$
\pagebreak

$\chi^{2}$
\pagebreak

\[ -log \mathcal{L} = N_{\mathrm{obs}} * \log(\lambda) - \sum_i^{N_{\mathrm{obs}}} \log(I(x_i)) \]
\pagebreak

$I(x_i)$
\pagebreak

$x_i$
\pagebreak

$ \lambda = \frac{V}{\sum w_i}\sum_i^{N_{\mathrm{phsp}}} I(x_i)\cdot \epsilon_i \cdot w_i $
\pagebreak

$ \epsilon $
\pagebreak

$ w $
\pagebreak

$ V $
\pagebreak

\[ \mathcal{A}_R(s) = \frac{g_p*g}{s - M_R^2 + i \sqrt{s} \Gamma_R B^2} \]
\pagebreak

$ g_p, g$
\pagebreak

$ B^2$
\pagebreak

\[ B^2 = \left( \frac{q(\sqrt{s})}{q(M_R)} \right)^{2L+1} \times \left( \frac{M_R}{\sqrt{s}} \right) \times \left( \frac{F(\sqrt{s})}{F(\sqrt{s_R})} \right)^{2} \]
\pagebreak

\[ B^2 = \left( \frac{q(\sqrt{s})}{q(M_R)} \right) \times \left( \frac{M_R}{\sqrt{s}} \right) \times \left( \frac{B_L(\sqrt{s})}{B_L(\sqrt{s_R})} \right)^{2} \]
\pagebreak

$m^2$
\pagebreak

$cos\Theta$
\pagebreak

$\phi$
\pagebreak

$f_1,f_2$
\pagebreak

$f_1$
\pagebreak

$f_2$
\pagebreak

$m^2, cos\Theta, \phi$
\pagebreak

$ M^{ij}_{\mu\nu\rho\ldots} $
\pagebreak

$ M^{ij}_{\mu\nu\rho\ldots} = mval^{ij} $
\pagebreak

$ g_{\mu\nu} $
\pagebreak

$ \left(\begin{array}{cccc} 1&0&0&0\\0&-1&0&0\\0&0&-1&0\\0&0&0&-1 \end{array}\right) $
\pagebreak

$\epsilon_{\mu\nu\rho\sigma}$
\pagebreak

$\vec{\beta}=(bx,by,bz)$
\pagebreak

$ X_{\mu\nu\ldots} = X_{\delta\pi\ldots} \Lambda^{\delta}{}_{\mu}(\vec{\beta})\Lambda^{\pi}{}_{\nu}(\vec{\beta}) \ldots $
\pagebreak

$ \alpha,\beta,\gamma $
\pagebreak

$ (\mu,\nu,\rho,\sigma,\delta,\pi) $
\pagebreak

$ R_{\mu_1\mu_2\ldots\nu_1\nu_2\ldots} = X_{\mu_1\mu_2\ldots\rho} T^{\rho}{}_{\nu_1\nu_2\ldots} $
\pagebreak

$ A_{\mu\nu} B^{\nu}{}_{\pi\delta} $
\pagebreak

$ R_{\rho\pi\ldots} = X_{\mu_1\mu_2\ldots} T^{\mu_1\mu_2\ldots}{}_{\rho\pi\ldots} $
\pagebreak

$ X_{\mu_1\mu_2\ldots\rho\pi\ldots} T^{\mu_1\mu_2\ldots} $
\pagebreak

$ A_{\mu\nu} B^{\mu\nu}{}_{\alpha} $
\pagebreak

$ R_{\mu_1\mu_2\ldots\nu_1\nu_2\ldots} = X_{\mu_1\mu_2\ldots} T{\nu_1\nu_2\ldots} $
\pagebreak

$ A_{\mu\nu} B_{\rho\pi\delta} $
\pagebreak

$ R_{\mu\nu\ldots} = X_{\mu\nu\ldots} \times x $
\pagebreak

$ R_{\mu\nu\ldots} = X_{\mu\nu\ldots} / x $
\pagebreak

$ R_{\mu\nu\ldots} = X_{\mu\nu\ldots} + T_{\mu\nu\ldots} $
\pagebreak

$ R_{\mu\nu\ldots} = X_{\mu\nu\ldots} - T_{\mu\nu\ldots} $
\pagebreak

$ A_{\rho\pi\mu\nu} $
\pagebreak

$ A = A_{\mu\nu\rho\pi} $
\pagebreak

$ R_{\mu_1\mu_2\ldots\nu_1\nu_2\ldots} = X_{\mu_1\mu_2\ldots\alpha_1\alpha_1\ldots\alpha_n} T^{\alpha_1\alpha_2\ldots\alpha_n}{}_{\nu_1\nu_2\ldots} $
\pagebreak

$ A_{\mu\nu} B^{\mu\nu\delta} $
\pagebreak

$ A^{\mu}{}_{\alpha} B^{\alpha\nu\delta} $
\pagebreak

$ A_{\rho\nu\mu} $
\pagebreak

$ A = A_{\mu\nu\rho} $
\pagebreak

$ A_{\mu\rho\nu} $
\pagebreak

$ (A_{\mu\nu\rho} + A_{\mu\rho\nu} + A_{\nu\mu\rho} + A_{\nu\rho\mu} + A_{\rho\mu\nu} + A_{\rho\nu\mu})/6.0 $
\pagebreak

$ (A_{\mu\nu\rho} - A_{\mu\rho\nu} - A_{\nu\mu\rho} + A_{\nu\rho\mu} + A_{\rho\mu\nu} - A_{\rho\nu\mu})/6.0 $
\pagebreak

$ X_{\mu\nu...} X^{\mu\nu...} $
\pagebreak

$ \Lambda^{\mu}{}_{\nu}$
\pagebreak

$ X_{\mu_1 \mu_2 ...} \Lambda^{\mu_1}{}_{\nu_1} \Lambda^{\mu_2}{}_{\nu_2} ... $
\pagebreak

$(\mu,\nu,...)$
\pagebreak

$ (\mu,\nu,\rho,...,\pi) $
\pagebreak

$ x_{\mu}, p_{\mu} $
\pagebreak

$ \beta \leq 1 $
\pagebreak

$\sqrt{px^2 + py^2 + pz^2}$
\pagebreak

$ \beta = \frac{p}{E} $
\pagebreak

$ \gamma = \frac{1}{\sqrt{1 - \beta^2}} $
\pagebreak

$ \sqrt{p_{\mu} p^{\mu}} $
\pagebreak

$ p_{\mu} p^{\mu} $
\pagebreak

$\sqrt{x^2 + y^2 + z^2}$
\pagebreak

$ \sqrt{x_{\mu} x^{\mu}} $
\pagebreak

$ x_{\mu} x^{\mu} $
\pagebreak

$ cos(\theta) = \frac{z}{r} $
\pagebreak

$\sqrt{x^2 + y^2}$
\pagebreak

$\sqrt{px^2 + py^2}$
\pagebreak

$ \theta = cos^{-1}(\frac{z}{r}) $
\pagebreak

$ \theta = tan^{-1}(\frac{y}{x}) $
\pagebreak

$ (-\pi,\pi) $
\pagebreak

$d^{j}_{m,n}(\beta)$
\pagebreak

$D^{j}_{m,n}(\alpha,\beta,\gamma)$
\pagebreak

\[ f_i = \frac{|c_i|^2 \int A_i A_i^*}{\int \sum c_l c_m^* A_l A_m^*} \]
\pagebreak

$c_i$
\pagebreak

$A_i$
\pagebreak

\[ f'(x) = \frac{f(x+h) - f(x-h)}{2h} + O(h^2) \]
\pagebreak

\[ \langle f \rangle =\frac{1}{N} \sum_{i=1}^N f(\overline{\mathbf{x}}_i) \]
\pagebreak

\[ I \approx Q_N = V*\langle f \rangle. \]
\pagebreak

\[ \mathrm{Var}(Q_N) = \frac{V^2}{N} \frac{1}{(N-1)} \sum_{i=1}^N \left (f(\overline{\mathbf{x}}_i) - \langle f \rangle \right )^2 \]
\pagebreak

\end{document}
